Examples.v
@@ -1,119 +1,57 @@
-From Coq Require Import Strings.String.
 From Coq Require Import Lists.List.
+From Coq Require Import Strings.String.
 Open Scope string_scope.
 
 From Elo Require Import Core.
+From Elo Require Import SyntacticProperties.
 From Elo Require Import Eval.
 
-(*
+Ltac solve_ty :=
+  repeat match goal with
+  | |- _ |-- <{unit                  }> is _ => eapply T_unit
+  | |- _ |-- <{nat _                 }> is _ => eapply T_nat
+  | |- _ |-- <{_; _                  }> is _ => eapply T_seq
+  | |- _ |-- <{if _ then _ else _ end}> is _ => eapply T_if
+  | |- _ |-- <{var _                 }> is _ => eapply T_var
+  | |- _ |-- <{fn _ _ _              }> is _ => eapply T_fun
+  | |- _ |-- <{call _ _              }> is _ => eapply T_call
+  | |- _ |-- <{new _ : r&?T          }> is _ => eapply T_newR
+  | |- _ |-- <{new _ : x&?T          }> is _ => eapply T_newX
+  | |- _ |-- <{new _ : w&?T          }> is _ => eapply T_newW
+  | |- _ |-- <{_ := _                }> is _ => eapply T_asg
+  | |- _ |-- <{acq _ _ _             }> is _ => eapply T_acq
+  | |- _ |-- <{reacq _               }> is _ => eapply T_reacq
+  | |- _ |-- <{spawn _               }> is _ => eapply T_spawn
+  end.
 
+Local Ltac solve_cw :=
+  repeat match goal with
+  | |- consistent_waits _ <{unit                  }> => eapply cw_unit
+  | |- consistent_waits _ <{nat _                 }> => eapply cw_nat
+  | |- consistent_waits _ <{_ + _                 }> => eapply cw_plus
+  | |- consistent_waits _ <{_ - _                 }> => eapply cw_monus
+  | |- consistent_waits _ <{_; _                  }> => eapply cw_seq
+  | |- consistent_waits _ <{if _ then _ else _ end}> => eapply cw_if
+  | |- consistent_waits _ <{while _ do _ end      }> => eapply cw_while
+  | |- consistent_waits _ <{var _                 }> => eapply cw_var
+  | |- consistent_waits _ <{fn _ _ _              }> => eapply cw_fun
+  | |- consistent_waits _ <{call _ _              }> => eapply cw_call
+  | |- consistent_waits _ <{new _ : _             }> => eapply cw_new
+  | |- consistent_waits _ <{init _ _ : _          }> => eapply cw_init
+  | |- consistent_waits _ <{* _                   }> => eapply cw_load
+  | |- consistent_waits _ <{_ := _                }> => eapply cw_asg
+  | |- consistent_waits _ <{acq _ _ _             }> => eapply cw_acq
+  | |- consistent_waits _ <{cr _ _                }> => eapply cw_cr
+  | |- consistent_waits _ <{reacq _               }> => eapply cw_reacq
+  | |- consistent_waits WR_self <{wait (var SELF) }> => eapply cw_wait1
+  | |- consistent_waits WR_ad _ <{wait (&_ : _)   }> => eapply cw_wait2
+  | |- consistent_waits _ <{reacq _               }> => eapply cw_reacq
+  | |- consistent_waits _ <{spawn _               }> => eapply cw_spawn
+  end.
 
-  tm_condwait   : list thread_id -> tm
-  tm_newcondvar : tm (* retorna um endereço pra tm_condwait *)
-  tm_broadcast  : tm -> tm
-  tm_wait       : tm -> tm
-
-  let down := fn m: (x&T) {
-    acq m p {
-      n := *p
-      while !n {
-        wait cv
-      }
-      n := n - 1
-    }
-  }
-
-
-  xpto ad --[e_reacq ad]--> unit
-
-
-  let up := fn m: (x&T) {
-    acq m p {
-      n := n + 1 
-      broadcast cv
-    }
-  }
-
-
-
-
-
-
-
-  wait a x ~~[tid, e_wait]~~>
-
-
-  while (!C) {
-   wait cv
-  }
-
-  signal cv
-  broadcast cv
-
-
-  wait-for-in C cv =
-    while (!C) {
-      rel
-      wait
-      acq
-    }
-
-
-
-  queroproduzir, queroconsumir
-
-  p:
-    down queroproduzir
-    enter CR
-      produz
-    leave CR
-    up queroconsumir
-
-  c:
-    down queroconsumir
-    enter CR
-      consume
-    leave CR
-    up queroproduzir
-
-
-
-
-*)
-
-
-
-(*
-  let m1 = new monitor(new w&Nat 3);
-  let m2 = new monitor(new w&Nat 5);
-  spawn {
-    acq m1 x {
-      let result = *x
-      x := 6
-      result
-    }
-  }
-  spawn {
-    acq m2 y {
-      let result = *y
-      x := 10
-      result
-    }
-  }
-  20
-
-
-  let m = new mon
-  acq m x {
-    ...
-    spawn {
-      acq m y {
-        ...
-      }
-    }
-  }
-
-*)
+(* ------------------------------------------------------------------------- *)
+(* example 1                                                                 *)
+(* ------------------------------------------------------------------------- *)
 
 Definition example1 : tm := <{
   let "m1" : x&w&Nat = new (new (nat 3) : w&Nat) : x&w&Nat in
@@ -138,40 +76,24 @@ Definition example1 : tm := <{
   )
 }>.
 
-Compute (last_result (evals nil (base example1) 200 0)).
+Compute (last_result (elo nil (base example1) 200 0)).
+
 (*
   m = (
-    [0]: (Some <{&1 : (w& Nat)}>, `x& (w& Nat) `, false, R_invalid) ::
-    [1]: (Some <{nat 6        }>, `w& Nat      `, false, R_invalid) ::
-    [2]: (Some <{&3 : (w& Nat)}>, `x& (w& Nat) `, false, R_invalid) ::
-    [3]: (Some <{nat 10       }>, `w& Nat      `, false, R_invalid) ::
-         nil
+    (Some <{&1 : (w& Nat) }>, `x&w& Nat)`, false, R_invalid) ::
+    (Some <{nat 6         }>, `w&Nat    `, false, R_invalid) ::
+    (Some <{&3 : (w& Nat) }>, `x&w& Nat)`, false, R_invalid) ::
+    (Some <{nat 10        }>, `w&Nat    `, false, R_invalid) ::
+    nil
   )
-  ths = (
-    [0]: <{nat 20 }> ::
-    [1]: <{nat 3  }> ::
-    [2]: <{nat 5  }> ::
-         nil
-  )
-  s = "out of gas"
-*)
 
-Ltac solve_ty :=
-  repeat match goal with
-  | |- _ |-- <{unit                  }> is _ => eapply T_unit
-  | |- _ |-- <{nat _                 }> is _ => eapply T_nat
-  | |- _ |-- <{_; _                  }> is _ => eapply T_seq
-  | |- _ |-- <{if _ then _ else _ end}> is _ => eapply T_if
-  | |- _ |-- <{var _                 }> is _ => eapply T_var
-  | |- _ |-- <{fn _ _ _              }> is _ => eapply T_fun
-  | |- _ |-- <{call _ _              }> is _ => eapply T_call
-  | |- _ |-- <{new _ : r&?T          }> is _ => eapply T_newR
-  | |- _ |-- <{new _ : x&?T          }> is _ => eapply T_newX
-  | |- _ |-- <{new _ : w&?T          }> is _ => eapply T_newW
-  | |- _ |-- <{_ := _                }> is _ => eapply T_asg
-  | |- _ |-- <{acq _ _ _             }> is _ => eapply T_acq
-  | |- _ |-- <{spawn _               }> is _ => eapply T_spawn
-  end.
+  ths = (
+    <{ nat 20 }> ::
+    <{ nat 3  }> ::
+    <{ nat 5  }> ::
+    nil
+  )
+*)
 
 Lemma example1_is_well_typed :
   empty |-- example1 is `Nat`.
@@ -188,44 +110,100 @@ Proof.
   - eapply T_loadW. solve_ty. rewrite lookup_update_eq. reflexivity.
 Qed.
 
-Lemma example1_reduces_correctly : forall m ths,
-  m = (
-    (Some <{nat 6     }>, `w&Nat`,   false, R_ad  1) ::
-    (Some <{&0 : w&Nat}>, `x&w&Nat`, false, R_tid 0) ::
-    (Some <{nat 10    }>, `w&Nat`,   false, R_ad  3) ::
-    (Some <{&2 : w&Nat}>, `x&w&Nat`, false, R_tid 0) ::
-    nil) -> 
-  ths = (
-    <{nat 6 }> ::
-    <{nat 10}> ::
-    <{nat 20}> ::
-    nil) ->
-  exists tc, nil \ (base example1) ~~[tc]~~>* m \ ths.
-Proof.
-  unfold base. intros. eexists.
-  eapply multistep_trans.
-Abort.
+Lemma example1_has_consistent_waits :
+  consistent_waits WR_none example1.
+Proof. unfold example1. solve_cw. Qed.
 
+(* ------------------------------------------------------------------------- *)
+(* example 2                                                                 *)
+(* ------------------------------------------------------------------------- *)
+
+Notation "'V`' x" := <{var x}>
+  (in custom elo_tm at level 0,
+           x constr at level 0).
+
+Notation "'N`' n" := <{nat n}>
+  (in custom elo_tm at level 0,
+           n constr at level 0).
+
+Definition example2 : tm := <{
+  let "bucket" : x&w&Nat = new (new (N`100) : w&Nat) : x&w&Nat in (
+    spawn (
+      while N`1 do
+        acq V`"bucket" "n" (
+          await *(V`"n");
+          V`"n" := *(V`"n") + N`1
+        )
+      end
+    );
+    spawn (
+      acq V`"bucket" "n" (
+        V`"n" := N`555
+      );
+      N`1337
+    )
+  )
+}>.
+
+Compute (last_result (elo nil (base example2) 5000 0)).
+
+(* gas = 10000
+
+  ((Some <{ &1 : w&Nat }>, `x&w& Nat `, true,  R_invalid)
+:: (Some <{ nat 555    }>, `w&Nat    `, false, R_invalid)
+:: nil)
+
+  (unit
+:: <{
+    cr 0 {
+      wait &0;
+      while *&1 do (wait (&0 : x&w&Nat) end);
+      &1 := *&1 + 1
+    };
+    while 1 do
+      acq &0 "n" {
+        await *n;
+        n := *n + 1
+      }
+    end
+    }>
+:: 1337
+:: nil)
+
+*)
 
 
 
 (*
-
-
-
-spawn {
-
-  while ? {
-    block
+  let down := fn m: (x&T) {
+    acq m p {
+      n := *p
+      while !n {
+        wait cv
+      }
+      n := n - 1
+    }
   }
 
-}
+  let up := fn m: (x&T) {
+    acq m p {
+      n := n + 1 
+      broadcast cv
+    }
+  }
 
+  p:
+    down queroproduzir
+    enter CR
+      produz
+    leave CR
+    up queroconsumir
 
-
-
-
-
-
-
+  c:
+    down queroconsumir
+    enter CR
+      consume
+    leave CR
+    up queroproduzir
 *)
+
