Safety.v
@@ -5,31 +5,44 @@ From Elo Require Import Core.
 From Elo Require Import SyntacticProperties.
 From Elo Require Import TypeProperties.
 
-From Elo Require Import Multistep.
-From Elo Require Import SafetyUtil.
-From Elo Require Import MemoryRegions.
+From Elo Require Import Invariants.
 From Elo Require Import GCR.
-From Elo Require Import HappensBefore.
 From Elo Require Import SafetyLemmas.
-From Elo Require Import SafetyGCR.
+From Elo Require Import SafetyUtil.
+From Elo Require Import HappensBefore.
 
 (* ------------------------------------------------------------------------- *)
+(* auxiliary - address                                                       *)
+(* ------------------------------------------------------------------------- *)
 
-Corollary ptyp_for_write_cstep : forall m1 m2 ths1 ths2 tid ad' t',
+Local Corollary read_address_cstep : forall m1 m2 ths1 ths2 tid ad' t',
+  m1 \ ths1 ~~[tid, e_read ad' t']~~> m2 \ ths2 ->
+  ad' < #m1.
+Proof.
+  intros. invc_cstep. invc_mstep.
+  lt_eq_gt ad' (#m2); sigma; trivial; discriminate.
+Qed.
+
+Local Corollary write_address_cstep : forall m1 m2 ths1 ths2 tid ad' t',
   invariants m1 ths1 ->
   (* --- *)
   m1 \ ths1 ~~[tid, e_write ad' t']~~> m2 \ ths2 ->
-  exists T, m1[ad'].T = `w&T`.
+  ad' < #m1.
 Proof.
-  intros. destruct_invariants. invc_cstep. invc_mstep.
-  eauto using ptyp_for_write. 
+  intros * Hinva ?.
+  eapply des_inva_vtm in Hinva. eapply des_forallprogram_threads in Hinva.
+  invc_cstep. invc_mstep. eauto using vtm_write_address.
 Qed.
 
-Lemma same_pointer_type :
+(* ------------------------------------------------------------------------- *)
+(* auxiliary - pointer types                                                 *)
+(* ------------------------------------------------------------------------- *)
+
+Local Corollary same_pointer_type :
   forall m1 mA mB m2 ths1 thsA thsB ths2 tc tid1 tid2 e1 e2 ad,
     invariants m1 ths1 ->
     (* --- *)
-    ad < #m1 ->
+    ad < #m1                             ->
     m1 \ ths1 ~~[tid1, e1]~~>  mA \ thsA ->
     mA \ thsA ~~[tc      ]~~>* mB \ thsB ->
     mB \ thsB ~~[tid2, e2]~~>  m2 \ ths2 ->
@@ -45,7 +58,84 @@ Proof.
   auto.
 Qed.
 
-Lemma same_regions :
+Local Corollary ptyp_for_write_cstep : forall m1 m2 ths1 ths2 tid ad' t',
+  invariants m1 ths1 ->
+  (* --- *)
+  m1 \ ths1 ~~[tid, e_write ad' t']~~> m2 \ ths2 ->
+  exists T, m1[ad'].T = `w&T`.
+Proof.
+  intros. destruct_invariants. invc_cstep. invc_mstep.
+  eauto using ptyp_for_write. 
+Qed.
+
+Local Corollary pointer_type_at_P1 :
+  forall m1 m2 mA mB ths1 ths2 thsA thsB tid1 tid2 tc ad t1 t2,
+    invariants m1 ths1 ->
+    invariants mB thsB ->
+    (* --- *)
+    m1 \ ths1 ~~[tid1, e_read  ad t1]~~>  mA \ thsA ->
+    mA \ thsA ~~[tc                 ]~~>* mB \ thsB ->
+    mB \ thsB ~~[tid2, e_write ad t2]~~>  m2 \ ths2 ->
+    exists T, m1[ad].T = `w&T`.
+Proof.
+  intros.
+  assert (ad < #m1) by eauto using read_address_cstep.
+  assert (exists T, mB[ad].T = `w&T`)
+    as [T HptypB]
+    by eauto using ptyp_for_write_cstep.
+  assert (m1[ad].T = mA[ad].T /\ mA[ad].T = mB[ad].T /\ mB[ad].T = m2[ad].T)
+    as [Hptyp1 [HptypA _]]
+    by eauto using same_pointer_type.
+  rewrite HptypB in HptypA.
+  rewrite HptypA in Hptyp1.
+  eauto.
+Qed.
+
+Local Corollary pointer_type_at_PB :
+  forall m1 m2 mA mB ths1 ths2 thsA thsB tid1 tid2 tc ad t1 t2,
+    invariants m1 ths1 ->
+    invariants mB thsB ->
+    (* --- *)
+    m1 \ ths1 ~~[tid1, e_write ad t1]~~>  mA \ thsA ->
+    mA \ thsA ~~[tc                 ]~~>* mB \ thsB ->
+    mB \ thsB ~~[tid2, e_read  ad t2]~~>  m2 \ ths2 ->
+    exists T, mB[ad].T = `w&T`.
+Proof.
+  intros.
+  assert (ad < #m1) by eauto using write_address_cstep.
+  assert (exists T, m1[ad].T = `w&T`)
+    as [T Hptyp1]
+    by eauto using ptyp_for_write_cstep.
+  assert (m1[ad].T = mA[ad].T /\ mA[ad].T = mB[ad].T /\ mB[ad].T = m2[ad].T)
+    as [HptypA [Hptyp2 _]]
+    by eauto using same_pointer_type.
+  rewrite Hptyp2 in HptypA.
+  rewrite HptypA in Hptyp1.
+  eauto.
+Qed.
+
+(* ------------------------------------------------------------------------- *)
+(* auxiliary - regions                                                       *)
+(* ------------------------------------------------------------------------- *)
+
+Local Lemma mreg_preservation_cstep : forall m1 m2 ths1 ths2 tid e ad,
+  ad < #m1                          ->
+  m1 \ ths1 ~~[tid, e]~~> m2 \ ths2 ->
+  m1[ad].R = m2[ad].R.
+Proof.
+  intros. invc_cstep; trivial; invc_mstep; sigma; trivial; omicron; trivial.
+Qed.
+
+Local Corollary mreg_preservation_ustep : forall m1 m2 ths1 ths2 tc ad,
+  ad < #m1                       ->
+  m1 \ ths1 ~~[tc]~~>* m2 \ ths2 ->
+  m1[ad].R = m2[ad].R.
+Proof.
+  intros. ind_ustep; trivial. rewrite IHmultistep;
+  eauto using ustep_nondecreasing_memory_size, mreg_preservation_cstep.
+Qed.
+
+Local Lemma same_regions :
   forall m1 mA mB m2 ths1 thsA thsB ths2 tc tid1 tid2 e1 e2 ad,
     invariants m1 ths1 ->
     (* --- *)
@@ -64,81 +154,8 @@ Proof.
   assumption.
 Qed.
 
-
 (* ------------------------------------------------------------------------- *)
-(* safety -- final 0                                                         *)
-(* ------------------------------------------------------------------------- *)
-
-Local Corollary write_address_cstep : forall m1 m2 ths1 ths2 tid ad' t',
-  invariants m1 ths1 ->
-  (* --- *)
-  m1 \ ths1 ~~[tid, e_write ad' t']~~> m2 \ ths2 ->
-  ad' < #m1.
-Proof.
-  intros * H ?.
-  eapply des_inva_vtm in H. eapply des_forallprogram_threads in H.
-  invc_cstep. invc_mstep. eauto using vtm_write_address.
-Qed.
-
-Local Corollary read_address_cstep : forall m1 m2 ths1 ths2 tid ad' t',
-  m1 \ ths1 ~~[tid, e_read ad' t']~~> m2 \ ths2 ->
-  ad' < #m1.
-Proof.
-  intros. invc_cstep. invc_mstep.
-  lt_eq_gt ad' (#m2); sigma; trivial; discriminate.
-Qed.
-
-Lemma todo1 : forall R m t ad,
-  valid_term m t ->
-  (* -- *)
-  R <> R_reacq ad      ->
-  gcr t R = R_reacq ad ->
-  waiting ad t.
-Proof.
-  intros. gendep R.
-  induction t; intros; invc_vtm; kappa; try discriminate;
-  eauto using waiting;
-  match goal with
-  | H : _ _ (R_ad ?ad) = _          |- _ => spec; specialize (IHt (R_ad ad))
-  | H : R_reacq ?ad1 = R_reacq ?ad2 |- _ => invc H
-  end;
-  auto using waiting with gcr.
-Qed.
-
-Lemma todo2 : forall m1 m2 ths1 ths2 tid ad ad' t',
-  waiting ad ths1[tid]                           ->
-  m1 \ ths1 ~~[tid, e_write ad' t']~~> m2 \ ths2 ->
-  False.
-Proof.
-  intros. invc_cstep. invc_mstep.
-  remember (ths1[tid]) as t1. clear Heqt1.
-  ind_tstep; repeat invc_wg; auto; (value_does_not_step || value_does_not_wait).
-Qed.
-
-Lemma todo2' : forall m1 m2 ths1 ths2 tid ad' t',
-  forall_threads ths1 (valid_term m1) ->
-  (* --- *)
-  m1 \ ths1 ~~[tid, e_write ad' t']~~> m2 \ ths2 ->
-  no_reacqs ths1[tid].
-Proof.
-  intros * Hvtm **. invc_cstep. invc_mstep.
-  specialize (Hvtm tid).
-  remember (ths1[tid]) as t1. clear Heqt1.
-  ind_tstep; invc_vtm; try value_does_not_step;
-  repeat spec; intro; eauto using noreacq_from_value, no_reacq.
-Qed.
-
-Corollary todo3 : forall m1 m2 ths1 ths2 tid ad ad' t',
-  forall_threads ths1 (valid_term m1) ->
-  (* --- *)
-  gcr ths1[tid] (R_tid tid) = R_reacq ad         ->
-  m1 \ ths1 ~~[tid, e_write ad' t']~~> m2 \ ths2 ->
-  False.
-Proof.
-  assert (forall tid ad, R_tid tid <> R_reacq ad) by congruence.
-  eauto using todo1, todo2.
-Qed.
-
+(* auxiliary - no-reacq                                                      *)
 (* ------------------------------------------------------------------------- *)
 
 Local Corollary noreacq_from_write_cstep :
@@ -161,11 +178,9 @@ Local Corollary noreacq_preservation_write_cstep :
     m1 \ ths1 ~~[tid, e_write ad' t']~~> m2 \ ths2 ->
     no_reacq ad ths2[tid].
 Proof.
-  intros * Hinva **. invc_cstep. invc_mstep. sigma. 
+  intros. invc_cstep. invc_mstep. sigma.
   eauto using noreacq_preservation_write.
 Qed.
-
-(* ------------------------------------------------------------------------- *)
 
 Local Corollary noreacq_from_read_cstep :
   forall m1 m2 ths1 ths2 tid ad' t' ad,
@@ -183,20 +198,88 @@ Qed.
 
 Local Corollary noreacq_preservation_read_cstep :
   forall m1 m2 ths1 ths2 tid ad' t' ad,
-    forall_memory m1 value           ->
-    forall_memory m1 (valid_term m1) ->
+    invariants m1 ths1 ->
     (* --- *)
     no_reacq ad ths1[tid]                         ->
     m1 \ ths1 ~~[tid, e_read ad' t']~~> m2 \ ths2 ->
     no_reacq ad ths2[tid].
 Proof.
-  intros * ? ? Hinva **. invc_cstep. invc_mstep. sigma. 
+  intros.
+  assert (forall_memory m1 value) by eauto with inva.
+  assert (forall_memory m1 (valid_term m1)) by eauto with inva.
+  invc_cstep. invc_mstep. sigma. 
   eauto using noreacq_from_value, noreacq_preservation_read.
 Qed.
 
 (* ------------------------------------------------------------------------- *)
-(* final three                                                               *)
+(* safety                                                                    *)
 (* ------------------------------------------------------------------------- *)
+
+Local Ltac solve_safety H1A HAB HB2 :=
+  (* Given the step relations. *)
+  match type of H1A with | ?m1 \ ?ths1 ~~[?tid1, ?e1 ?ad _]~~>  ?mA \ ?thsA =>
+  match type of HAB with | ?mA \ ?thsA ~~[?tc             ]~~>* ?mB \ ?thsB =>
+  match type of HB2 with | ?mB \ ?thsB ~~[?tid2, ?e2 ?ad _]~~>  ?m2 \ ?ths2 =>
+
+    (* Asserts the invariants for PA, PB, and P2. *)
+    assert (invariants mA thsA) by eauto using invariants_preservation_cstep;
+    assert (invariants mB thsB) by eauto using invariants_preservation_ustep;
+    assert (invariants m2 ths2) by eauto using invariants_preservation_cstep;
+
+    (* Analyzes the first effect. *)
+    match e1 with
+    | e_read =>
+      (* If the first effect is a READ, asserts the pointer type. *)
+      (* Lemma cstep_gcr_read requires it. *)
+      assert (exists T, m1[ad].T = `w&T`) as [T ?]
+        by eauto using pointer_type_at_P1;
+      (* Then gets the current region for P1. *)
+      assert (HgcrA : gcr ths1[tid1] (R_tid tid1) = m1[ad].R)
+        by eauto using cstep_gcr_read with inva;
+      (* And for PA by preservation. *)
+      erewrite (gcr_preservation_read_cstep m1 mA ths1 thsA) in HgcrA;
+      eauto with inva
+    | e_write =>
+      (* If the first effect is a WRITE, gets the current region for P1. *)
+      assert (HgcrA : gcr ths1[tid1] (R_tid tid1) = m1[ad].R)
+        by eauto 7 using cstep_gcr_write with inva;
+      (* And for PA by preservation. *)
+      erewrite gcr_preservation_write_cstep in HgcrA; eauto with inva
+    end;
+
+    (* Analyzes the second effect. *)
+    match e2 with
+    | e_read =>
+      (* If the second effect is a READ, asserts the pointer type. *)
+      (* Lemma cstep_gcr_read requires it. *)
+      assert (exists T, mB[ad].T = `w&T`) as [T ?]
+        by eauto using pointer_type_at_PB;
+      (* Then gets the current region for PB. *)
+      assert (HgcrB : gcr thsB[tid2] (R_tid tid2) = mB[ad].R)
+        by eauto using cstep_gcr_read with inva
+    | e_write =>
+      (* If the second effect is a WRITE, gets the current region for PB. *)
+      assert (HgcrB : gcr thsB[tid2] (R_tid tid2) = mB[ad].R)
+        by eauto 7 using cstep_gcr_write with inva
+    end;
+
+    (* Asserts both PA and PB are in the same region. *)
+    assert (HR : m1[ad].R = mB[ad].R)
+      by eauto using read_address_cstep, write_address_cstep, same_regions;
+    rewrite <- HR in *;
+
+    (* Analyzes the region in which PA and PB are in. *)
+    destruct (m1[ad].R);
+    (* A thread cannot be in an invalid region. *)
+    try solve [exfalso; eauto using gcr_invalid_contradiction];
+    (* Two different threads cannot be in the same thread region. *)
+    try solve [exfalso; eauto using gcr_tid_contradiction];
+
+    (* The two threads are in a monitored region. *)
+    eapply (happens_before_from_gcr mA mB thsA thsB); eauto
+  end
+  end
+  end.
 
 Theorem safety_write_write : forall m1 m2 ths1 ths2 tc tc' tid1 tid2 ad t1 t2,
   invariants m1 ths1 ->
@@ -206,40 +289,9 @@ Theorem safety_write_write : forall m1 m2 ths1 ths2 tc tc' tid1 tid2 ad t1 t2,
   happens_before tc.
 Proof.
   intros. subst.
-  nat_eq_dec tid1 tid2; eauto using happens_before.
-
-  destruct_ustep2.
-  assert (invariants mA thsA) by eauto using invariants_preservation_cstep.
-  assert (invariants mB thsB) by eauto using invariants_preservation_ustep.
-  assert (invariants m2 ths2) by eauto using invariants_preservation_cstep.
-
-  assert (ad < #m1) by eauto using write_address_cstep.
-
-  assert (exists T, m1[ad].T = `w&T`)
-    as [T Hptyp1]
-    by eauto using ptyp_for_write_cstep.
-  assert (m1[ad].T = mA[ad].T /\ mA[ad].T = mB[ad].T /\ mB[ad].T = m2[ad].T)
-    as [HptypA [HptypB Hptyp2]]
-    by eauto using same_pointer_type.
-  rewrite Hptyp1 in HptypA. symmetry in HptypA.
-  rewrite HptypA in HptypB. symmetry in HptypB.
-  rewrite HptypB in Hptyp2. symmetry in Hptyp2.
-
-  assert (Hgcr1 : gcr ths1[tid1] (R_tid tid1) = m1[ad].R)
-    by eauto 7 using cstep_gcr_write with inva.
-  assert (HgcrB : gcr thsB[tid2] (R_tid tid2) = mB[ad].R)
-    by eauto 7 using cstep_gcr_write with inva.
-
-  assert (HR : m1[ad].R = mB[ad].R) by eauto using same_regions.
-  rewrite <- HR in *.
-
-  destruct (m1[ad].R).
-  - exfalso. eauto using gcr_tid_contradiction with gcr.
-  - exfalso. eauto using gcr_tid_contradiction with gcr.
-  - erewrite gcr_preservation_write_cstep in Hgcr1; eauto with inva.
-    eapply (happens_before_from_gcr mA mB thsA thsB);
-    eauto using noreacq_from_write_cstep, noreacq_preservation_write_cstep.
-  - exfalso. eauto using todo3 with inva.
+  nat_eq_dec tid1 tid2; eauto using happens_before. destruct_ustep2.
+  solve_safety H1A HAB HB2;
+  eauto using noreacq_from_write_cstep, noreacq_preservation_write_cstep.
 Qed.
 
 Theorem safety_write_read : forall m1 m2 ths1 ths2 tc tc' tid1 tid2 ad t1 t2,
@@ -250,41 +302,10 @@ Theorem safety_write_read : forall m1 m2 ths1 ths2 tc tc' tid1 tid2 ad t1 t2,
   happens_before tc.
 Proof.
   intros. subst.
-  nat_eq_dec tid1 tid2; eauto using happens_before.
-
-  destruct_ustep2.
-  assert (invariants mA thsA) by eauto using invariants_preservation_cstep.
-  assert (invariants mB thsB) by eauto using invariants_preservation_ustep.
-  assert (invariants m2 ths2) by eauto using invariants_preservation_cstep.
-
-  assert (ad < #m1) by eauto using write_address_cstep.
-
-  assert (exists T, m1[ad].T = `w&T`)
-    as [T Hptyp1]
-    by eauto using ptyp_for_write_cstep.
-  assert (m1[ad].T = mA[ad].T /\ mA[ad].T = mB[ad].T /\ mB[ad].T = m2[ad].T)
-    as [HptypA [HptypB Hptyp2]]
-    by eauto using same_pointer_type.
-  rewrite Hptyp1 in HptypA. symmetry in HptypA.
-  rewrite HptypA in HptypB. symmetry in HptypB.
-  rewrite HptypB in Hptyp2. symmetry in Hptyp2.
-
-  assert (Hgcr1 : gcr ths1[tid1] (R_tid tid1) = m1[ad].R)
-    by eauto 7 using cstep_gcr_write with inva.
-  assert (HgcrB : gcr thsB[tid2] (R_tid tid2) = mB[ad].R)
-    by eauto using cstep_gcr_read with inva.
-
-  assert (HR : m1[ad].R = mB[ad].R) by eauto using same_regions.
-  rewrite <- HR in *.
-
-  destruct (m1[ad].R).
-  - exfalso. eauto using gcr_tid_contradiction with gcr.
-  - exfalso. eauto using gcr_tid_contradiction with gcr.
-  - erewrite gcr_preservation_write_cstep in Hgcr1; eauto with inva.
-    eapply (happens_before_from_gcr mA mB thsA thsB); eauto;
-    eauto using noreacq_from_read_cstep;
-    eauto using noreacq_from_write_cstep, noreacq_preservation_write_cstep.
-  - exfalso. eauto using todo3 with inva.
+  nat_eq_dec tid1 tid2; eauto using happens_before. destruct_ustep2.
+  solve_safety H1A HAB HB2;
+  eauto using noreacq_from_write_cstep, noreacq_preservation_write_cstep.
+  eauto using noreacq_from_read_cstep.
 Qed.
 
 Theorem safety_read_write : forall m1 m2 ths1 ths2 tc tc' tid1 tid2 ad t1 t2,
@@ -295,43 +316,9 @@ Theorem safety_read_write : forall m1 m2 ths1 ths2 tc tc' tid1 tid2 ad t1 t2,
   happens_before tc.
 Proof.
   intros. subst.
-  nat_eq_dec tid1 tid2; eauto using happens_before.
-
-  destruct_ustep2.
-  assert (invariants mA thsA) by eauto using invariants_preservation_cstep.
-  assert (invariants mB thsB) by eauto using invariants_preservation_ustep.
-  assert (invariants m2 ths2) by eauto using invariants_preservation_cstep.
-
-  assert (ad < #m1) by eauto using read_address_cstep.
-
-  assert (exists T, mB[ad].T = `w&T`)
-    as [T HptypB]
-    by eauto using ptyp_for_write_cstep.
-  assert (m1[ad].T = mA[ad].T /\ mA[ad].T = mB[ad].T /\ mB[ad].T = m2[ad].T)
-    as [Hptyp1 [HptypA Hptyp2]]
-    by eauto using same_pointer_type.
-  rewrite HptypB in HptypA.
-  rewrite HptypA in Hptyp1.
-  rewrite HptypB in Hptyp2.
-  symmetry in Hptyp2.
-
-  assert (Hgcr1 : gcr ths1[tid1] (R_tid tid1) = m1[ad].R)
-    by eauto using cstep_gcr_read with inva.
-  assert (HgcrB : gcr thsB[tid2] (R_tid tid2) = mB[ad].R)
-    by eauto 7 using cstep_gcr_write with inva.
-
-  assert (HR : m1[ad].R = mB[ad].R) by eauto using same_regions.
-  rewrite <- HR in *.
-
-  destruct (m1[ad].R).
-  - exfalso. eauto using gcr_tid_contradiction with gcr.
-  - exfalso. eauto using gcr_tid_contradiction with gcr.
-  - erewrite (gcr_preservation_read_cstep m1 mA ths1 thsA) in Hgcr1;
-    eauto with inva.
-    eapply (happens_before_from_gcr mA mB thsA thsB); eauto;
-    eauto using noreacq_from_write_cstep.
-    eapply (noreacq_preservation_read_cstep m1 mA ths1 thsA); eauto with inva.
-    eauto using noreacq_from_read_cstep.
-  - exfalso. eauto using todo3 with inva.
+  nat_eq_dec tid1 tid2; eauto using happens_before. destruct_ustep2.
+  solve_safety H1A HAB HB2;
+  eauto using noreacq_from_write_cstep.
+  eauto using noreacq_from_read_cstep, noreacq_preservation_read_cstep.
 Qed.
 
